Verification infrastructure of GOTO_on_List programs: 1. determinismus 2. behaviour when no modification 3. behaviour when no jump 4. behaviour when each variable modified only once, with its dependent variables unmodified before the modification to itself (incomplete)

IMPminus_TM/TM_GOTO/GOTO_on_List.thy
@@ -68,21 +68,26 @@ fun iexec\<^sub>l :: "GOTO\<^sub>l_instr \<Rightarrow> config\<^sub>l \<Rightarr
   "iexec\<^sub>l (MoveRight n) (pc, s) = (Suc pc, s(HP n := [Suc (hd (s (HP n)))]))" |
   "iexec\<^sub>l (GOTO\<^sub>l label) (pc, s) = (label, s)" |
   "iexec\<^sub>l (IF x = l THEN GOTO\<^sub>l label) (pc, s) =
-    (if (s x = eval_GOTO\<^sub>l_operi s l) then label else pc, s)" |
-  "iexec\<^sub>l (IF x = l1 AND y = l2 THEN GOTO\<^sub>l label) (pc, s) =
-    (if s x = eval_GOTO\<^sub>l_operi s l1 \<and> s y = eval_GOTO\<^sub>l_operi s l2 then label else pc, s)"
+    (if (s x = eval_GOTO\<^sub>l_operi s l) then label else Suc pc, s)" |
+  "iexec\<^sub>l (IF x = l\<^sub>1 AND y = l\<^sub>2 THEN GOTO\<^sub>l label) (pc, s) =
+    (if s x = eval_GOTO\<^sub>l_operi s l\<^sub>1 \<and> s y = eval_GOTO\<^sub>l_operi s l\<^sub>2 then label else Suc pc, s)"
 
 definition exec1\<^sub>l :: "GOTO\<^sub>l_prog \<Rightarrow> config\<^sub>l \<Rightarrow> config\<^sub>l \<Rightarrow> bool" ("(_/ \<turnstile>\<^sub>l (_ \<rightarrow>/ _))" [59,0,59] 60) where
   "P \<turnstile>\<^sub>l cfg \<rightarrow> cfg' \<longleftrightarrow> (\<exists>pc s. cfg = (pc, s) \<and> cfg' = iexec\<^sub>l (P !! pc) cfg \<and>
-                         P \<noteq> [] \<and> 0 < pc \<and> pc \<le> size P)"
+                         P \<noteq> [] \<and> 0 < pc \<and> pc \<le> length P)"
 
 text \<open>Note that pc = 0 is when the program halts\<close>
 lemma exec1\<^sub>l_I [intro, code_pred_intro]:
-  "c' = iexec\<^sub>l (P !! pc) (pc, s) \<Longrightarrow> P \<noteq> [] \<Longrightarrow> 0 < pc \<Longrightarrow> pc \<le> size P \<Longrightarrow> P \<turnstile>\<^sub>l (pc, s) \<rightarrow> c'"
+  "c' = iexec\<^sub>l (P !! pc) (pc, s) \<Longrightarrow> P \<noteq> [] \<Longrightarrow> 0 < pc \<Longrightarrow> pc \<le> length P \<Longrightarrow>
+   P \<turnstile>\<^sub>l (pc, s) \<rightarrow> c'"
   by (simp add: exec1\<^sub>l_def of_nat_diff)
 
 lemma exec1\<^sub>l_pc_range [intro]:
   "P \<turnstile>\<^sub>l (pc, s) \<rightarrow> c' \<Longrightarrow> 0 < pc \<and> pc \<le> length P"
+  unfolding exec1\<^sub>l_def by blast
+
+lemma exec1\<^sub>l_iexec\<^sub>l [intro]:
+  "P \<turnstile>\<^sub>l (pc, s) \<rightarrow> c' \<Longrightarrow> iexec\<^sub>l (P !! pc) (pc, s) = c'"
   unfolding exec1\<^sub>l_def by blast
 
 abbreviation
@@ -127,39 +132,274 @@ values
 
 
 subsection \<open>Verification infrastructure\<close>
-text \<open>This part draws largely on "HOL-IMP.Compiler"\<close>
 
-fun ins_no_jump :: "state\<^sub>l \<Rightarrow> GOTO\<^sub>l_instr \<Rightarrow> bool" where
-  "ins_no_jump s ins \<longleftrightarrow> (
-    (\<nexists>n. ins = GOTO\<^sub>l n) \<and>
-    (\<exists>x l n. ins = IF x = l THEN GOTO\<^sub>l n \<longrightarrow> s x \<noteq> eval_GOTO\<^sub>l_operi s l) \<and>
-    (\<exists>x y l\<^sub>1 l\<^sub>2 n. (ins = IF x = l\<^sub>1 AND y = l\<^sub>1 THEN GOTO\<^sub>l n) \<longrightarrow>
-         (s x \<noteq> eval_GOTO\<^sub>l_operi s l\<^sub>1 \<or> s y \<noteq> eval_GOTO\<^sub>l_operi s l\<^sub>2)))"
+text \<open>The program is executed deterministically\<close>
+lemma iexec\<^sub>l_determ [intro]:
+  "iexec\<^sub>l ins s = s\<^sub>1 \<Longrightarrow> iexec\<^sub>l ins s = s\<^sub>2 \<Longrightarrow> s\<^sub>1 = s\<^sub>2"
+  by (cases ins) auto
 
-lemma iexec\<^sub>l_seq_independent_from_pc[simp]:
-  assumes "ins_no_jump s ins"
-    shows "iexec\<^sub>l ins (pc, s) = (pc', s') \<Longrightarrow> \<forall>pc''. iexec\<^sub>l ins (pc, s) = (pc', s')"
-  using assms
-  by (auto split: GOTO\<^sub>l_instr.split)
+lemma exec1\<^sub>l_determ [intro]:
+  "P \<turnstile>\<^sub>l cfg \<rightarrow> cfg' \<Longrightarrow> P \<turnstile>\<^sub>l cfg \<rightarrow> cfg'' \<Longrightarrow> cfg' = cfg''"
+  unfolding exec1\<^sub>l_def
+  by blast
 
-lemma exec1\<^sub>l_appendR:
-  assumes "ins_no_jump s (P!!pc)"
-    shows "P \<turnstile>\<^sub>l (pc, s) \<rightarrow> c' \<Longrightarrow> P @ P' \<turnstile>\<^sub>l (pc, s) \<rightarrow> c'"
-  by (auto simp: exec1\<^sub>l_def)
-
-lemma exec_appendR:
-  assumes "\<forall>ins \<in> set P. ins_no_jump s ins"
-    shows "P \<turnstile>\<^sub>l (pc, s) \<rightarrow>* c'' \<Longrightarrow> P @ P' \<turnstile>\<^sub>l (pc, s) \<rightarrow>* c''"
-proof (induction "(pc, s)" c'' rule: star.induct)
-  case refl
-  then show ?case by blast
+lemma exec\<^sub>l_t_determ [intro]:
+  "P \<turnstile>\<^sub>l cfg \<rightarrow>\<^bsub>t\<^esub> cfg' \<Longrightarrow> P \<turnstile>\<^sub>l cfg \<rightarrow>\<^bsub>t\<^esub> cfg'' \<Longrightarrow> cfg' = cfg''"
+proof (induction t arbitrary: cfg)
+  case 0
+  then show ?case by auto
 next
-  case (step c' c'')
-  with exec1\<^sub>l_pc_range have "0 < pc \<and> pc \<le> length P" by blast
-  then have "P !! pc \<in> set P" by blast
-  with assms have "ins_no_jump s (P !! pc)" by blast
-  with step exec1\<^sub>l_appendR have "P @ P' \<turnstile>\<^sub>l (pc, s) \<rightarrow> c'" by blast
-  with step show ?case  sorry
+  case (Suc t)
+  from Suc obtain cfg\<^sub>1 where cfg\<^sub>1: "P \<turnstile>\<^sub>l cfg \<rightarrow> cfg\<^sub>1" "P \<turnstile>\<^sub>l cfg\<^sub>1 \<rightarrow>\<^bsub>t\<^esub> cfg'"
+    by (metis relpowp_Suc_D2)
+  from Suc obtain cfg\<^sub>2 where cfg\<^sub>2: "P \<turnstile>\<^sub>l cfg \<rightarrow> cfg\<^sub>2" "P \<turnstile>\<^sub>l cfg\<^sub>2 \<rightarrow>\<^bsub>t\<^esub> cfg''"
+    by (metis relpowp_Suc_D2)
+  from \<open>P \<turnstile>\<^sub>l cfg \<rightarrow> cfg\<^sub>1\<close> \<open>P \<turnstile>\<^sub>l cfg \<rightarrow> cfg\<^sub>2\<close> have "cfg\<^sub>1 = cfg\<^sub>2" by fast
+  with Suc.IH \<open>P \<turnstile>\<^sub>l cfg\<^sub>1 \<rightarrow>\<^bsub>t\<^esub> cfg'\<close> \<open>P \<turnstile>\<^sub>l cfg\<^sub>2 \<rightarrow>\<^bsub>t\<^esub> cfg''\<close>
+  show ?case by blast
+qed
+
+text \<open>The verification of GOTO on List programs depends on very specific properties of the program,
+below are some lemmas about the behaviour of the program with certain properties.\<close>
+
+text \<open>First, a large part of the transformed program does not contain modification to any variable.
+This is a very useful information for verification.\<close>
+
+fun no_modification :: "GOTO\<^sub>l_instr \<Rightarrow> bool" where
+  "no_modification (_ ::=\<^sub>l _) \<longleftrightarrow> False" |
+  "no_modification (TapeModify _ _) \<longleftrightarrow> False" |
+  "no_modification (MoveLeft _) \<longleftrightarrow> False" |
+  "no_modification (MoveRight _) \<longleftrightarrow> False" |
+  "no_modification _ \<longleftrightarrow> True"
+
+lemma iexec\<^sub>l_no_modification[intro]:
+  assumes "no_modification ins"
+    shows "\<exists>pc'. iexec\<^sub>l ins (pc, s) = (pc', s)"
+  using assms
+  by (cases ins) auto
+
+text \<open>If a block of program contains no jump command, or only conditional jumps
+with conditions unsatisfied under the given state, the block is then executed sequentially.
+With this information, the runtime can be determined directly.\<close>
+
+fun no_jump :: "state\<^sub>l \<Rightarrow> GOTO\<^sub>l_instr \<Rightarrow> bool" where
+  "no_jump s HALT\<^sub>l \<longleftrightarrow> False" | \<comment>\<open>HALT \<equiv> GOTO 0\<close>
+  "no_jump s (GOTO\<^sub>l _) \<longleftrightarrow> False" |
+  "no_jump s (IF x = l THEN GOTO\<^sub>l _) \<longleftrightarrow> s x \<noteq> eval_GOTO\<^sub>l_operi s l" |
+  "no_jump s (IF x = l\<^sub>1 AND y = l\<^sub>2 THEN GOTO\<^sub>l _) \<longleftrightarrow>
+   s x \<noteq> eval_GOTO\<^sub>l_operi s l\<^sub>1 \<or> s y \<noteq> eval_GOTO\<^sub>l_operi s l\<^sub>2" |
+  "no_jump _ _ \<longleftrightarrow> True"
+
+lemma iexec\<^sub>l_no_jump[intro]:
+  assumes "no_jump s ins"
+    shows "\<exists>s'. iexec\<^sub>l ins (pc, s) = (Suc pc, s')"
+  using assms
+  by (cases ins) auto
+
+fun strict_no_jump :: "GOTO\<^sub>l_instr \<Rightarrow> bool" where
+  "strict_no_jump HALT\<^sub>l \<longleftrightarrow> False" | \<comment>\<open>HALT \<equiv> GOTO 0\<close>
+  "strict_no_jump (GOTO\<^sub>l _) \<longleftrightarrow> False" |
+  "strict_no_jump (IF x = l THEN GOTO\<^sub>l _) \<longleftrightarrow> False" |
+  "strict_no_jump (IF x = l\<^sub>1 AND y = l\<^sub>2 THEN GOTO\<^sub>l _) \<longleftrightarrow> False" |
+  "strict_no_jump _ \<longleftrightarrow> True"
+
+lemma strict_no_jump_no_jump[intro]:
+  "strict_no_jump ins \<Longrightarrow> \<forall>s. no_jump s ins"
+  by (cases ins) auto
+
+lemma iexec\<^sub>l_strict_no_jump[intro]:
+  assumes "strict_no_jump ins"
+    shows "\<exists>s'. iexec\<^sub>l ins (pc, s) = (Suc pc, s')"
+  using assms
+  by (cases ins) auto
+
+lemma execute_prog_strict_no_jump:
+  assumes block_P_a_len: "0 < a \<and> a + len \<le> length P \<and> P \<noteq> []"
+      and block_strict_no_jump: "\<forall>i. a \<le> i \<and> i < a + len \<longrightarrow> strict_no_jump (P !! i)"
+    shows "\<exists>s'. P \<turnstile>\<^sub>l (a, s) \<rightarrow>\<^bsub>len\<^esub> (a + len, s')"
+  using assms
+proof (induction len)
+  case 0
+  then show ?case by simp
+next
+  case (Suc len)
+  then obtain s' where "P \<turnstile>\<^sub>l (a, s) \<rightarrow>\<^bsub>len\<^esub> (a + len, s')" by auto
+  moreover
+  from Suc.prems have "strict_no_jump (P !! (a + len))" by simp
+  then obtain s'' where "iexec\<^sub>l (P !! (a + len)) (a + len, s') = (a + Suc len, s'')" by force
+  then have "P \<turnstile>\<^sub>l (a + len, s') \<rightarrow> (a + Suc len, s'')" using Suc by auto
+  ultimately
+  show ?case by auto
+qed
+
+lemma execute_prog_strict_no_jump_mid_state:
+  assumes block_P_a_len: "0 < a \<and> a + Suc len \<le> length P \<and> P \<noteq> []"
+      and block_strict_no_jump: "\<forall>i. a \<le> i \<and> i < a + Suc len \<longrightarrow> strict_no_jump (P !! i)"
+      and final_state: "P \<turnstile>\<^sub>l (a, s) \<rightarrow>\<^bsub>Suc len\<^esub> (a + Suc len, t)"
+    shows "\<exists>t'. (P \<turnstile>\<^sub>l (a, s) \<rightarrow>\<^bsub>len\<^esub> (a + len, t')) \<and> (P \<turnstile>\<^sub>l (a + len, t') \<rightarrow> (a + Suc len, t))"
+proof -
+  from block_P_a_len block_strict_no_jump
+  obtain t' where t': "P \<turnstile>\<^sub>l (a, s) \<rightarrow>\<^bsub>len\<^esub> (a + len, t')"
+    using execute_prog_strict_no_jump by fastforce
+  from block_strict_no_jump have "strict_no_jump (P !! (a + len))" by auto
+  with t' have "P \<turnstile>\<^sub>l (a + len, t') \<rightarrow> (a + Suc len, t)"
+    by (metis exec\<^sub>l_t_determ final_state relpowp_Suc_E)
+  with t' show ?thesis by blast
+qed
+
+text \<open>In the best situation, a block of program runs sequentially and the state remains the same.
+This is luckily the case for the entrance block in the transformed program.\<close>
+lemma iexec\<^sub>l_no_jump_and_no_modification[intro]:
+  assumes "no_jump s ins" 
+      and "no_modification ins"
+    shows "iexec\<^sub>l ins (pc, s) = (Suc pc, s)"
+  using assms
+  by (cases ins) auto
+
+lemma execute_prog_no_jump_and_no_modification:
+  "0 < a \<and> a + len \<le> length P \<Longrightarrow> P \<noteq> [] \<Longrightarrow>
+   \<forall>i. a \<le> i \<and> i < a + len \<longrightarrow> no_jump s (P !! i) \<and> no_modification (P !! i) \<Longrightarrow>
+   P \<turnstile>\<^sub>l (a, s) \<rightarrow>\<^bsub>len\<^esub> (a + len, s)"
+proof (induction len)
+  case 0
+  then show ?case by auto
+next
+  case (Suc len)
+  then have "P \<turnstile>\<^sub>l (a, s) \<rightarrow>\<^bsub>len\<^esub> (a + len, s)" by force
+  moreover
+  from Suc.prems have "no_jump s (P !! (a + len))" "no_modification (P !! (a + len))" by simp+
+  then have "iexec\<^sub>l (P !! (a + len)) (a + len, s) = (a + Suc len, s)" by auto
+  then have "P \<turnstile>\<^sub>l (a + len, s) \<rightarrow> (a + Suc len, s)" using Suc by auto
+  ultimately
+  show ?case by auto
+qed
+
+text \<open>Another informative situation is when the program runs sequentially, and some variable
+is modified at most once. In this case the value of variable can be inferred statically
+from the commands in the program block.\<close>
+
+fun no_write :: "var\<^sub>l \<Rightarrow> GOTO\<^sub>l_instr \<Rightarrow> bool" where
+  \<comment>\<open>ST, the state of the Turing Machine\<close>
+  "no_write ST (x ::=\<^sub>l l) \<longleftrightarrow> x \<noteq> ST" |
+  "no_write ST _ \<longleftrightarrow> True" |
+  \<comment>\<open>TP n, the n-th tape of the Turing Machine\<close>
+  "no_write (TP n) (x ::=\<^sub>l l) \<longleftrightarrow> x \<noteq> TP n" |
+  "no_write (TP n) (TapeModify m v) \<longleftrightarrow> n \<noteq> m" |
+  "no_write (TP n) _ \<longleftrightarrow> True" |
+  \<comment>\<open>HP n, head position of the n-th tape of the Turing Machine\<close>
+  "no_write (HP n) (x ::=\<^sub>l l) \<longleftrightarrow> x \<noteq> HP n" |
+  "no_write (HP n) (MoveLeft m) \<longleftrightarrow> m \<noteq> n" |
+  "no_write (HP n) (MoveRight m) \<longleftrightarrow> m \<noteq> n" |
+  "no_write (HP n) _ \<longleftrightarrow> True" |
+  \<comment>\<open>TMP n, other variables used in the program\<close>
+  "no_write (TMP n) (x ::=\<^sub>l l) \<longleftrightarrow> x \<noteq> TMP n" |
+  "no_write (TMP n) _ \<longleftrightarrow> True"
+
+lemma iexec\<^sub>l_no_write[intro]:
+  assumes "no_write x ins"
+      and "iexec\<^sub>l ins (pc, s) = (pc', s')"
+    shows "s' x = s x"
+  using assms
+  by (cases ins; cases x) auto
+
+lemma execute_no_write_and_strict_no_jump:
+  assumes block_P_a_len: "0 < a \<and> a + len \<le> length P \<and> P \<noteq> []"
+      and block_strict_no_jump_and_no_write:
+          "\<forall>i. a \<le> i \<and> i < a + len \<longrightarrow> strict_no_jump (P !! i) \<and> no_write x (P !! i)"
+      and final_state: "P \<turnstile>\<^sub>l (a, s) \<rightarrow>\<^bsub>len\<^esub> (a + len, s')"
+    shows "s' x = s x"
+  using assms
+proof (induction len arbitrary: s')
+  case 0
+  then show ?case by auto
+next
+  case (Suc len)
+  then have IH_cond: "0 < a \<and> a + len \<le> length P" "P \<noteq> []"
+    "\<forall>i. a \<le> i \<and> i < a + len \<longrightarrow> strict_no_jump (P !! i) \<and> no_write x (P !! i)"
+    by simp+
+  with execute_prog_strict_no_jump obtain s_mid where s_mid: "P \<turnstile>\<^sub>l (a, s) \<rightarrow>\<^bsub>len\<^esub> (a + len, s_mid)"
+    by blast
+  with Suc.IH IH_cond have "s_mid x = s x" by blast
+  moreover
+  from Suc have prop_cur_ins: "strict_no_jump (P !! (a + len)) \<and> no_write x (P !! (a + len))" by auto
+  then obtain s'' where s'': "P \<turnstile>\<^sub>l (a + len, s_mid) \<rightarrow> (a + Suc len, s'')"
+    by (metis Suc.prems(3) exec\<^sub>l_t_determ relpowp_Suc_E s_mid)
+  with prop_cur_ins have "s'' x = s_mid x" by blast
+  moreover
+  from s_mid s'' have "P \<turnstile>\<^sub>l (a, s) \<rightarrow>\<^bsub>Suc len\<^esub> (a + Suc len, s'')"
+    by auto
+  with \<open>P \<turnstile>\<^sub>l (a, s) \<rightarrow>\<^bsub>Suc len\<^esub> (a + Suc len, s')\<close> have "s' = s''" 
+    using exec\<^sub>l_t_determ [where ?t = "Suc len"] by blast
+  ultimately
+  show ?case by simp
+qed
+
+fun vars_read_in_operi :: "GOTO\<^sub>l_operi \<Rightarrow> var\<^sub>l set" where
+  "vars_read_in_operi (L l) = {}" |
+  "vars_read_in_operi (V\<^sub>l y) = {y}" |
+  "vars_read_in_operi (ReadChs tps) = (TP ` (set tps)) \<union> (HP ` (set tps))"
+
+fun vars_read :: "GOTO\<^sub>l_instr \<Rightarrow> var\<^sub>l set" where
+  "vars_read (x ::=\<^sub>l l) = vars_read_in_operi l" |
+  "vars_read (TapeModify n v) = {TP n, HP n}" |
+  "vars_read (MoveLeft n) = {HP n}" |
+  "vars_read (MoveRight n) = {HP n}" |
+  "vars_read (IF x = l THEN GOTO\<^sub>l label) = vars_read_in_operi l \<union> {x}" |
+  "vars_read (IF x = l\<^sub>1 AND y = l\<^sub>2 THEN GOTO\<^sub>l label) =
+     vars_read_in_operi l\<^sub>1 \<union> {x} \<union> vars_read_in_operi l\<^sub>2 \<union> {y}" |
+  "vars_read _ = {}"
+
+lemma iexec\<^sub>l_with_all_dependent_var_same:
+  assumes "\<forall>y \<in> vars_read ins. s y = s' y"
+      and "s x = s' x"
+      and "iexec\<^sub>l ins (pc, s) = (pc', t)"
+      and "iexec\<^sub>l ins (pc, s') = (pc', t')"
+    shows "t x = t' x"
+  using assms
+  apply (cases ins)
+  apply auto
+  subgoal for operi
+    by (cases operi) auto
+  done
+
+lemma execute_with_var_modified_at_most_once:
+  assumes block_P_a_len: "0 < a \<and> a + len \<le> length P \<and> P \<noteq> []"
+      \<comment>\<open>ins_modify: the only possible point where x is modified\<close>
+      and ins_modify: "0 \<le> j \<and> j < len \<and> (P !! j) = ins_modify"
+      and "strict_no_jump ins_modify"
+      and state_before_ins_modify: "P \<turnstile>\<^sub>l (a, s) \<rightarrow>\<^bsub>j\<^esub> (a + j, s')"
+      and state_after_ins_modify: "P \<turnstile>\<^sub>l (a + j, s') \<rightarrow> (a + j', s'')"
+      and value_x: "s'' x = v"
+      and other_cmd_no_write_x: "\<forall>i. a \<le> i \<and> i < a + len \<and> i \<noteq> j \<longrightarrow> strict_no_jump (P !! i) \<and> no_write x (P !! i)"
+      and config_at_end: "P \<turnstile>\<^sub>l (a, s) \<rightarrow>\<^bsub>len\<^esub> (a + len, t)"
+    shows "t x = v"
+  using assms
+proof (induction len)
+  case 0
+  then show ?case by linarith
+next
+  case (Suc len)
+  then have strict_no_jump: "\<forall>i. a \<le> i \<and> i < a + Suc len \<longrightarrow> strict_no_jump (P !! i)"
+    by blast
+  with \<open>0 < a \<and> a + Suc len \<le> length P \<and> P \<noteq> []\<close> \<open>P \<turnstile>\<^sub>l (a, s) \<rightarrow>\<^bsub>Suc len\<^esub> (a + Suc len, t)\<close>
+  obtain t' where t': "P \<turnstile>\<^sub>l (a, s) \<rightarrow>\<^bsub>len\<^esub> (a + len, t')" "P \<turnstile>\<^sub>l (a + len, t') \<rightarrow> (a + Suc len, t)"
+    using execute_prog_strict_no_jump_mid_state by blast
+
+  show ?case
+  proof (cases "j = a + len")
+    case True \<comment>\<open>variable x can only be modified at (P !! (a + len)), not before\<close>
+    with Suc have "\<forall>i. a \<le> i \<and> i < a + len \<longrightarrow> strict_no_jump (P !! i) \<and> no_write x (P !! i)"
+      using dual_order.strict_trans by blast
+    with Suc t' have "t' x = s x"
+      using execute_no_write_and_strict_no_jump
+      by (metis Suc_leD add_Suc_right)
+    from t' True have "P \<turnstile>\<^sub>l (j, t') \<rightarrow> (a + Suc len, t)" by blast
+    then show ?thesis sorry
+  next
+    case False \<comment>\<open>variable x can only be modified at (P !! j), which is before (P !! (a + len))\<close>
+    with Suc
+    show ?thesis sorry
+  qed
 qed
 
 end
